infoflow: PasUpdates arch split
Signed-off-by: Ryan Barry <ryan.barry@unsw.edu.au>

proof/infoflow/PasUpdates.thy
@@ -12,64 +12,64 @@ text \<open>
 
 theory PasUpdates
 imports
-    "Arch_IF"
+    "ArchArch_IF"
     "FinalCaps"
     "AInvs.EmptyFail_AI"
 begin
 
-context begin interpretation Arch . (*FIXME: arch_split*)
-
 section \<open>Separation lemmas for the idle thread and domain fields\<close>
 
-abbreviation (input) domain_fields
-where
+abbreviation (input) domain_fields where
   "domain_fields P s \<equiv> P (domain_time s) (domain_index s) (domain_list s)"
 
 lemma preemption_point_domain_fields[wp]:
-  "\<lbrace>domain_fields P\<rbrace> preemption_point \<lbrace>\<lambda>_. domain_fields P\<rbrace>"
+  "preemption_point \<lbrace>domain_fields P\<rbrace>"
   by (simp add: preemption_point_def
       | wp OR_choiceE_weak_wp modify_wp
       | wpc
       | simp add: reset_work_units_def update_work_units_def)+
 
-crunch domain_fields[wp]: retype_region_ext,create_cap_ext,cap_insert_ext,ethread_set,
-                          cap_move_ext,empty_slot_ext,cap_swap_ext,set_thread_state_ext,
-                          tcb_sched_action,reschedule_required,cap_swap_for_delete,
-                          finalise_cap,cap_move,cap_swap,cap_delete,cancel_badged_sends,
-                          cap_insert
-                          "domain_fields P"
+
+locale PasUpdates_1 =
+  fixes aag :: "'a subject_label PAS"
+  assumes arch_post_cap_deletion_domain_fields[wp]:
+    "arch_post_cap_deletion acap \<lbrace>domain_fields P\<rbrace>"
+  and arch_finalise_cap_domain_fields[wp]:
+    "arch_finalise_cap acap b \<lbrace>domain_fields P\<rbrace>"
+  and prepare_thread_delete_domain_fields[wp]:
+    "prepare_thread_delete p \<lbrace>domain_fields P\<rbrace>"
+begin
+
+crunch domain_fields[wp]:
+  retype_region_ext, create_cap_ext, cap_insert_ext, ethread_set, cap_move_ext, empty_slot_ext,
+  cap_swap_ext, set_thread_state_ext, tcb_sched_action, reschedule_required, cap_swap_for_delete,
+  finalise_cap, cap_move, cap_swap, cap_delete, cancel_badged_sends, cap_insert
+  "domain_fields P"
   (    wp: syscall_valid select_wp crunch_wps rec_del_preservation cap_revoke_preservation modify_wp
      simp: crunch_simps check_cap_at_def filterM_mapM unless_def
    ignore: without_preemption filterM rec_del check_cap_at cap_revoke
    ignore_del: retype_region_ext create_cap_ext cap_insert_ext ethread_set cap_move_ext
                empty_slot_ext cap_swap_ext set_thread_state_ext tcb_sched_action reschedule_required)
 
-lemma cap_revoke_domain_fields[wp]:"\<lbrace>domain_fields P\<rbrace> cap_revoke a \<lbrace>\<lambda>_. domain_fields P\<rbrace>"
+lemma cap_revoke_domain_fields[wp]:
+  "cap_revoke a \<lbrace>domain_fields P\<rbrace>"
   by (rule cap_revoke_preservation2; wp)
 
-lemma invoke_cnode_domain_fields[wp]: "\<lbrace>domain_fields P\<rbrace> invoke_cnode a \<lbrace>\<lambda>_. domain_fields P\<rbrace>"
+lemma invoke_cnode_domain_fields[wp]:
+  "invoke_cnode a \<lbrace>domain_fields P\<rbrace>"
   unfolding invoke_cnode_def
-  by (wpsimp wp: get_cap_wp hoare_vcg_all_lift hoare_vcg_imp_lift
-      | rule conjI)+
+  by (wpsimp wp: get_cap_wp hoare_vcg_all_lift hoare_vcg_imp_lift | rule conjI)+
 
-crunch domain_fields[wp]:
-  set_domain,possible_switch_to,set_priority,set_extra_badge,
-  handle_send,handle_recv,handle_reply
-  "domain_fields P"
-  (wp: syscall_valid crunch_wps mapME_x_inv_wp
-   simp: crunch_simps check_cap_at_def detype_def detype_ext_def mapM_x_defsym
-   ignore: check_cap_at syscall
-   ignore_del: set_domain set_priority possible_switch_to
-   rule: transfer_caps_loop_pres)
+end
+
 
 section \<open>PAS wellformedness property for non-interference\<close>
 
 definition pas_wellformed_noninterference where
   "pas_wellformed_noninterference aag \<equiv>
-    (\<forall>l\<in>range (pasObjectAbs aag) \<union> \<Union>(range (pasDomainAbs aag)) - {SilcLabel}.
-         pas_wellformed (aag\<lparr> pasSubject := l \<rparr>)) \<and>
-    (\<forall>d. SilcLabel \<notin> pasDomainAbs aag d) \<and>
-    pas_domains_distinct aag"
+     (\<forall>l \<in> range (pasObjectAbs aag) \<union> \<Union>(range (pasDomainAbs aag)) - {SilcLabel}.
+        pas_wellformed (aag\<lparr>pasSubject := l\<rparr>)) \<and>
+     (\<forall>d. SilcLabel \<notin> pasDomainAbs aag d) \<and> pas_domains_distinct aag"
 
 lemma pas_wellformed_noninterference_domains_distinct:
   "pas_wellformed_noninterference aag \<Longrightarrow> pas_domains_distinct aag"
@@ -77,160 +77,149 @@ lemma pas_wellformed_noninterference_domains_distinct:
 
 lemma pas_wellformed_noninterference_silc[intro!]:
   "pas_wellformed_noninterference aag \<Longrightarrow> SilcLabel \<notin> pasDomainAbs aag d"
-  apply (fastforce simp: pas_wellformed_noninterference_def)
-  done
+  by (fastforce simp: pas_wellformed_noninterference_def)
+
 
 section \<open>PAS subject update\<close>
 
 lemma pasObjectAbs_pasSubject_update:
-  "pasObjectAbs (aag\<lparr> pasSubject := x \<rparr>) = pasObjectAbs aag"
-  apply simp
-  done
+  "pasObjectAbs (aag\<lparr>pasSubject := x\<rparr>) = pasObjectAbs aag"
+  by simp
 
 lemma pasASIDAbs_pasSubject_update:
-  "pasASIDAbs (aag\<lparr> pasSubject := x \<rparr>) = pasASIDAbs aag"
-  apply simp
-  done
+  "pasASIDAbs (aag\<lparr>pasSubject := x\<rparr>) = pasASIDAbs aag"
+  by simp
 
 lemma pasIRQAbs_pasSubject_update:
-  "pasIRQAbs (aag\<lparr> pasSubject := x \<rparr>) = pasIRQAbs aag"
-  apply simp
-  done
-
-lemma state_asids_to_policy_pasSubject_update:
-  "state_asids_to_policy_aux (aag\<lparr> pasSubject := x \<rparr>) caps asid vrefs =
-   state_asids_to_policy_aux aag caps asid vrefs"
-  apply(rule equalityI)
-   apply(clarify)
-   apply(erule state_asids_to_policy_aux.cases
-        |simp
-        |fastforce intro: state_asids_to_policy_aux.intros)+
-  apply(clarify)
-  apply(erule state_asids_to_policy_aux.cases)
-   apply(simp,
-         subst pasObjectAbs_pasSubject_update[symmetric],
-         subst pasASIDAbs_pasSubject_update[symmetric],
-         rule state_asids_to_policy_aux.intros, assumption+)+
-  done
+  "pasIRQAbs (aag\<lparr>pasSubject := x\<rparr>) = pasIRQAbs aag"
+  by simp
 
 lemma state_irqs_to_policy_pasSubject_update:
-  "state_irqs_to_policy_aux (aag\<lparr> pasSubject := x \<rparr>) caps =
+  "state_irqs_to_policy_aux (aag\<lparr>pasSubject := x\<rparr>) caps =
    state_irqs_to_policy_aux aag caps"
-  apply(rule equalityI)
-   apply(clarify)
-   apply(erule state_irqs_to_policy_aux.cases, simp,
-         blast intro: state_irqs_to_policy_aux.intros)
-  apply(clarify)
-  apply(erule state_irqs_to_policy_aux.cases)
-  apply(simp)
-  apply(subst pasObjectAbs_pasSubject_update[symmetric])
-  apply(subst pasIRQAbs_pasSubject_update[symmetric])
-  apply(rule state_irqs_to_policy_aux.intros)
+  apply (rule equalityI; clarify)
+   apply (erule state_irqs_to_policy_aux.cases, simp, blast intro: state_irqs_to_policy_aux.intros)
+  apply (erule state_irqs_to_policy_aux.cases)
+  apply simp
+  apply (subst pasObjectAbs_pasSubject_update[symmetric])
+  apply (subst pasIRQAbs_pasSubject_update[symmetric])
+  apply (rule state_irqs_to_policy_aux.intros)
    apply assumption+
   done
 
-
 lemma irq_map_wellformed_pasSubject_update:
-  "irq_map_wellformed_aux (aag\<lparr> pasSubject := x \<rparr>) irqn =
+  "irq_map_wellformed_aux (aag\<lparr>pasSubject := x\<rparr>) irqn =
    irq_map_wellformed_aux aag irqn"
   by (clarsimp simp: irq_map_wellformed_aux_def)
 
 lemma tcb_domain_map_wellformed_pasSubject_update:
-  "tcb_domain_map_wellformed_aux (aag\<lparr> pasSubject := x \<rparr>) irqn =
+  "tcb_domain_map_wellformed_aux (aag\<lparr>pasSubject := x\<rparr>) irqn =
    tcb_domain_map_wellformed_aux aag irqn"
   by (clarsimp simp: tcb_domain_map_wellformed_aux_def)
 
+
+locale PasUpdates_2 = PasUpdates_1 +
+  assumes arch_perform_invocation_domain_fields[wp]:
+    "arch_perform_invocation i \<lbrace>domain_fields P\<rbrace>"
+  and arch_invoke_irq_control_domain_fields[wp]:
+    "arch_invoke_irq_control ci \<lbrace>domain_fields P\<rbrace>"
+  and arch_invoke_irq_handler_domain_fields[wp]:
+    "arch_invoke_irq_handler hi \<lbrace>domain_fields P\<rbrace>"
+  and arch_post_modify_registers_domain_fields[wp]:
+    "arch_post_modify_registers cur t \<lbrace>domain_fields P\<rbrace>"
+  and handle_arch_fault_reply_domain_fields[wp]:
+    "handle_arch_fault_reply vmf thread x y \<lbrace>domain_fields P\<rbrace>"
+  and init_arch_objects_domain_fields[wp]:
+    "init_arch_objects typ ptr num sz refs \<lbrace>domain_fields P\<rbrace>"
+  and state_asids_to_policy_pasSubject_update:
+    "state_asids_to_policy (aag\<lparr>pasSubject := subject\<rparr>) s =
+     state_asids_to_policy aag s"
+  and state_asids_to_policy_pasMayActivate_update:
+    "state_asids_to_policy (aag\<lparr>pasMayActivate := b\<rparr>) s =
+     state_asids_to_policy aag s"
+  and state_asids_to_policy_pasMayEditReadyQueues_update:
+    "state_asids_to_policy (aag\<lparr>pasMayEditReadyQueues := b\<rparr>) s =
+     state_asids_to_policy aag s"
+begin
+
+crunch domain_fields[wp]:
+  set_domain,possible_switch_to,set_priority,set_extra_badge,handle_send,handle_recv,handle_reply
+  "domain_fields P"
+  (wp: syscall_valid crunch_wps mapME_x_inv_wp
+   simp: crunch_simps check_cap_at_def detype_def detype_ext_def mapM_x_defsym
+   ignore: check_cap_at syscall
+   ignore_del: set_domain set_priority possible_switch_to
+   rule: transfer_caps_loop_pres)
+
 lemma pas_refined_pasSubject_update':
-   "\<lbrakk>pas_refined aag s; pas_wellformed (aag\<lparr> pasSubject := x \<rparr>)\<rbrakk> \<Longrightarrow>
-   pas_refined (aag\<lparr> pasSubject := x \<rparr>) s"
-  apply(subst pas_refined_def)
-  apply(safe del: subsetI)
+  "\<lbrakk> pas_refined aag s; pas_wellformed (aag\<lparr>pasSubject := x\<rparr>) \<rbrakk>
+     \<Longrightarrow> pas_refined (aag\<lparr>pasSubject := x\<rparr>) s"
+  apply (subst pas_refined_def)
+  apply (safe del: subsetI)
       apply (simp add: irq_map_wellformed_pasSubject_update pas_refined_def)
      apply (simp add: tcb_domain_map_wellformed_pasSubject_update pas_refined_def)
     apply (clarsimp simp: pas_refined_def)
-   apply(fastforce simp: pas_refined_def state_asids_to_policy_pasSubject_update)
-  apply(fastforce simp: pas_refined_def state_irqs_to_policy_pasSubject_update)
+   apply (clarsimp simp: pas_refined_def state_asids_to_policy_pasSubject_update)
+  apply (fastforce simp: pas_refined_def state_irqs_to_policy_pasSubject_update)
   done
 
 lemma pas_wellformed_pasSubject_update:
-  "\<lbrakk>pas_wellformed_noninterference aag; l \<in> pasDomainAbs aag d\<rbrakk> \<Longrightarrow>
-   pas_wellformed (aag\<lparr>pasSubject := l\<rparr>)"
+  "\<lbrakk> pas_wellformed_noninterference aag; l \<in> pasDomainAbs aag d \<rbrakk>
+     \<Longrightarrow> pas_wellformed (aag\<lparr>pasSubject := l\<rparr>)"
   by (auto simp: pas_wellformed_noninterference_def)
 
 lemmas pas_refined_pasSubject_update =
-                   pas_refined_pasSubject_update'[OF _ pas_wellformed_pasSubject_update]
+  pas_refined_pasSubject_update'[OF _ pas_wellformed_pasSubject_update]
+
+end
+
 
 lemma guarded_pas_domain_pasSubject_update[simp]:
   "guarded_pas_domain (aag\<lparr>pasSubject := x\<rparr>) s = guarded_pas_domain aag s"
   by (simp add: guarded_pas_domain_def)
 
-
 lemma silc_inv_pasSubject_update':
-  "\<lbrakk>silc_inv aag st s; x \<noteq> SilcLabel\<rbrakk> \<Longrightarrow> silc_inv (aag\<lparr>pasSubject := x\<rparr>) st s"
+  "\<lbrakk> silc_inv aag st s; x \<noteq> SilcLabel \<rbrakk>
+     \<Longrightarrow> silc_inv (aag\<lparr>pasSubject := x\<rparr>) st s"
   by (auto simp: silc_inv_def silc_dom_equiv_def intra_label_cap_def cap_points_to_label_def)
 
 lemma silc_inv_pasSubject_update:
-  "\<lbrakk>silc_inv aag st s; pas_wellformed_noninterference aag; l \<in> pasDomainAbs aag d\<rbrakk>
-   \<Longrightarrow> silc_inv (aag\<lparr>pasSubject := l\<rparr>) st s"
-  apply (fastforce intro: silc_inv_pasSubject_update' dest: pas_wellformed_noninterference_silc)
-  done
+  "\<lbrakk> silc_inv aag st s; pas_wellformed_noninterference aag; l \<in> pasDomainAbs aag d \<rbrakk>
+     \<Longrightarrow> silc_inv (aag\<lparr>pasSubject := l\<rparr>) st s"
+  by (fastforce intro: silc_inv_pasSubject_update' dest: pas_wellformed_noninterference_silc)
+
 
 section \<open>PAS MayActivate update\<close>
 
 lemma prop_of_pasMayActivate_update_idemp:
-  "\<lbrakk>P aag; pasMayActivate aag = v\<rbrakk> \<Longrightarrow> P (aag\<lparr> pasMayActivate := v \<rparr>)"
+  "\<lbrakk> P aag; pasMayActivate aag = v \<rbrakk> \<Longrightarrow> P (aag\<lparr>pasMayActivate := v\<rparr>)"
   by (hypsubst, auto)
 
 lemma pasObjectAbs_pasMayActivate_update:
-  "pasObjectAbs (aag\<lparr> pasMayActivate := x \<rparr>) = pasObjectAbs aag"
+  "pasObjectAbs (aag\<lparr>pasMayActivate := x\<rparr>) = pasObjectAbs aag"
   by simp
 
 lemma pasASIDAbs_pasMayActivate_update:
-  "pasASIDAbs (aag\<lparr> pasMayActivate := x \<rparr>) = pasASIDAbs aag"
+  "pasASIDAbs (aag\<lparr>pasMayActivate := x\<rparr>) = pasASIDAbs aag"
   by simp
 
 lemma pasIRQAbs_pasMayActivate_update:
-  "pasIRQAbs (aag\<lparr> pasMayActivate := x \<rparr>) = pasIRQAbs aag"
+  "pasIRQAbs (aag\<lparr>pasMayActivate := x\<rparr>) = pasIRQAbs aag"
   by simp
 
-lemma state_asids_to_policy_pasMayActivate_update:
-  "state_asids_to_policy (aag\<lparr> pasMayActivate := x \<rparr>) s =
-   state_asids_to_policy aag s"
-  apply(rule equalityI)
-   apply(clarify)
-   apply(erule state_asids_to_policy_aux.cases
-        |simp
-        |fastforce intro: state_asids_to_policy_aux.intros)+
-  apply(clarify)
-  apply(erule state_asids_to_policy_aux.cases)
-   apply(simp,
-         subst pasObjectAbs_pasMayActivate_update[symmetric],
-         subst pasASIDAbs_pasMayActivate_update[symmetric],
-         rule state_asids_to_policy_aux.intros, assumption+)+
-  done
-
 lemma state_irqs_to_policy_pasMayActivate_update:
-  "state_irqs_to_policy (aag\<lparr> pasMayActivate := x \<rparr>) s =
+  "state_irqs_to_policy (aag\<lparr>pasMayActivate := x\<rparr>) s =
    state_irqs_to_policy aag s"
-  apply(rule equalityI)
-   apply(clarify)
-   apply(erule state_irqs_to_policy_aux.cases
-        |simp
-        |fastforce intro: state_irqs_to_policy_aux.intros)+
-  apply(clarify)
-  apply(erule state_irqs_to_policy_aux.cases)
-   apply(simp,
-         subst pasObjectAbs_pasMayActivate_update[symmetric],
-         subst pasIRQAbs_pasMayActivate_update[symmetric],
-         rule state_irqs_to_policy_aux.intros, assumption+)+
-  done
-
-lemma pas_refined_pasMayActivate_update:
-  "pas_refined aag s \<Longrightarrow>
-   pas_refined (aag\<lparr> pasMayActivate := x \<rparr>) s"
-  apply(simp add: pas_refined_def)
-  apply(clarsimp simp: irq_map_wellformed_aux_def state_asids_to_policy_pasMayActivate_update[simplified]
-                       state_irqs_to_policy_pasMayActivate_update tcb_domain_map_wellformed_aux_def)
+  apply (rule equalityI)
+   apply (clarify)
+   apply (erule state_irqs_to_policy_aux.cases
+          | simp
+          | fastforce intro: state_irqs_to_policy_aux.intros)+
+  apply (clarify)
+  apply (erule state_irqs_to_policy_aux.cases)
+  apply (simp, subst pasObjectAbs_pasMayActivate_update[symmetric]
+             , subst pasIRQAbs_pasMayActivate_update[symmetric]
+             , rule state_irqs_to_policy_aux.intros, assumption+)
   done
 
 lemma guarded_pas_domainMayActivate_update[simp]:
@@ -238,69 +227,62 @@ lemma guarded_pas_domainMayActivate_update[simp]:
   by (simp add: guarded_pas_domain_def)
 
 lemma cdt_change_allowedMayActivate_update[simp]:
-  "cdt_change_allowed (aag\<lparr>pasMayActivate := x\<rparr>) =
-   cdt_change_allowed aag "
+  "cdt_change_allowed (aag\<lparr>pasMayActivate := x\<rparr>) = cdt_change_allowed aag "
   by (simp add: cdt_change_allowed_def[abs_def] cdt_direct_change_allowed.simps direct_call_def)
+
 
 section \<open>PAS MayEditReadyQueue update\<close>
 
 lemma prop_of_pasMayEditReadyQueues_update_idemp:
-  "\<lbrakk>P aag; pasMayEditReadyQueues aag = v\<rbrakk> \<Longrightarrow> P (aag\<lparr> pasMayEditReadyQueues := v \<rparr>)"
+  "\<lbrakk> P aag; pasMayEditReadyQueues aag = v \<rbrakk> \<Longrightarrow> P (aag\<lparr>pasMayEditReadyQueues := v\<rparr>)"
   by clarsimp
 
 lemma pasObjectAbs_pasMayEditReadyQueues_update:
-  "pasObjectAbs (aag\<lparr> pasMayEditReadyQueues := x \<rparr>) = pasObjectAbs aag"
+  "pasObjectAbs (aag\<lparr>pasMayEditReadyQueues := x\<rparr>) = pasObjectAbs aag"
   by simp
 
 lemma pasASIDAbs_pasMayEditReadyQueues_update:
-  "pasASIDAbs (aag\<lparr> pasMayEditReadyQueues := x \<rparr>) = pasASIDAbs aag"
+  "pasASIDAbs (aag\<lparr>pasMayEditReadyQueues := x\<rparr>) = pasASIDAbs aag"
   by simp
 
 lemma pasIRQAbs_pasMayEditReadyQueues_update:
-  "pasIRQAbs (aag\<lparr> pasMayEditReadyQueues := x \<rparr>) = pasIRQAbs aag"
+  "pasIRQAbs (aag\<lparr>pasMayEditReadyQueues := x\<rparr>) = pasIRQAbs aag"
   by simp
 
-lemma state_asids_to_policy_pasMayEditReadyQueues_update:
-  "state_asids_to_policy (aag\<lparr> pasMayEditReadyQueues := x \<rparr>) s =
-   state_asids_to_policy aag s"
-  apply(rule equalityI)
-   apply(clarify)
-   apply(erule state_asids_to_policy_aux.cases
-        |simp
-        |fastforce intro: state_asids_to_policy_aux.intros)+
-  apply(clarify)
-  apply(erule state_asids_to_policy_aux.cases)
-   apply(simp,
-         subst pasObjectAbs_pasMayEditReadyQueues_update[symmetric],
-         subst pasASIDAbs_pasMayEditReadyQueues_update[symmetric],
-         rule state_asids_to_policy_aux.intros, assumption+)+
+lemma state_irqs_to_policy_pasMayEditReadyQueues_update:
+  "state_irqs_to_policy (aag\<lparr>pasMayEditReadyQueues := x\<rparr>) s =
+   state_irqs_to_policy aag s"
+  apply (rule equalityI)
+   apply (clarify)
+   apply (erule state_irqs_to_policy_aux.cases
+          | simp
+          | fastforce intro: state_irqs_to_policy_aux.intros)+
+  apply (clarify)
+  apply (erule state_irqs_to_policy_aux.cases)
+  apply (simp, subst pasObjectAbs_pasMayEditReadyQueues_update[symmetric]
+             , subst pasIRQAbs_pasMayEditReadyQueues_update[symmetric]
+             , rule state_irqs_to_policy_aux.intros, assumption+)
   done
 
-lemma state_irqs_to_policy_pasMayEditReadyQueues_update:
-  "state_irqs_to_policy (aag\<lparr> pasMayEditReadyQueues := x \<rparr>) s =
-   state_irqs_to_policy aag s"
-  apply(rule equalityI)
-   apply(clarify)
-   apply(erule state_irqs_to_policy_aux.cases
-        |simp
-        |fastforce intro: state_irqs_to_policy_aux.intros)+
-  apply(clarify)
-  apply(erule state_irqs_to_policy_aux.cases)
-   apply(simp,
-         subst pasObjectAbs_pasMayEditReadyQueues_update[symmetric],
-         subst pasIRQAbs_pasMayEditReadyQueues_update[symmetric],
-         rule state_irqs_to_policy_aux.intros, assumption+)+
-  done
+
+context PasUpdates_2 begin
+
+lemma pas_refined_pasMayActivate_update:
+  "pas_refined aag s
+   \<Longrightarrow> pas_refined (aag\<lparr>pasMayActivate := x\<rparr>) s"
+  by (simp add: pas_refined_def irq_map_wellformed_aux_def
+                state_asids_to_policy_pasMayActivate_update[simplified]
+                state_irqs_to_policy_pasMayActivate_update tcb_domain_map_wellformed_aux_def)
 
 lemma pas_refined_pasMayEditReadyQueues_update:
-  "pas_refined aag s \<Longrightarrow>
-   pas_refined (aag\<lparr> pasMayEditReadyQueues := x \<rparr>) s"
-  apply(simp add: pas_refined_def)
-  apply(clarsimp simp: irq_map_wellformed_aux_def
-                       state_asids_to_policy_pasMayEditReadyQueues_update[simplified]
-                       state_irqs_to_policy_pasMayEditReadyQueues_update
-                       tcb_domain_map_wellformed_aux_def)
-  done
+  "pas_refined aag s
+   \<Longrightarrow> pas_refined (aag\<lparr>pasMayEditReadyQueues := x\<rparr>) s"
+  by (clarsimp simp: pas_refined_def irq_map_wellformed_aux_def tcb_domain_map_wellformed_aux_def
+                     state_asids_to_policy_pasMayEditReadyQueues_update[simplified]
+                     state_irqs_to_policy_pasMayEditReadyQueues_update)
+
+end
+
 
 lemma guarded_pas_domainMayEditReadyQueues_update[simp]:
   "guarded_pas_domain (aag\<lparr>pasMayEditReadyQueues := False\<rparr>) = guarded_pas_domain aag"
@@ -310,7 +292,5 @@ lemma cdt_change_allowedMayEditReadyQueues_update[simp]:
   "cdt_change_allowed (aag\<lparr>pasMayEditReadyQueues := x\<rparr>) =
    cdt_change_allowed aag"
   by (simp add: cdt_change_allowed_def[abs_def] cdt_direct_change_allowed.simps direct_call_def)
-
-end
 
 end
